tests/wip/concept_param_mismatch/concept_param_mismatch.t.cpp
@@ -1,0 +1,10 @@
+// Copyright 2026 Bloomberg Finance L.P.
+// Distributed under the terms of the GNU LGPL v2.1 license.
+#include "concept_param_mismatch.h"
+#include <iostream>
+
+int main() {
+  auto r = ConceptParamMismatch::test;
+  std::cout << (r == 6 ? "PASSED" : "FAILED") << std::endl;
+  return r != 6; 
+}
